# Circle Through Three Points

![circle](./img/2b6b4095-290a-4547-81b1-6fce09861b17.svg)

```math
\begin{align*}
\left( x-c_x\right)^2+\left( y-c_y\right)^2 &= r^2 \
 x^2-2c_x x + c_x^2 + y^2 -2c_y y + c_y^2 &= r^2 \
-2c_x x - 2c_y y + c_x^2 + c_y^2 -r^2 &= -\left(x^2+y^2\right) \
A x + B y + C = -\left(x^2+y^2\right)
\end{align*}
```
Where $A=-2c_x$, $B=-2c_y$ and $C=c_x^2 + c_y^2 -r^2$.
Rearanging these we get
```math
\begin{align*}
c_x&=-\frac{A}{2}\
c_y&=-\frac{B}{2}\
r&=\frac{1}{2}\sqrt{A^2+B^2-4C}
\end{align*}
```
