\begin{equation} 
r=\lambda^3 a + \lambda^2 b + \lambda c +d
\end{equation}
\begin{equation} 
\frac{d r}{d\lambda}=3\lambda^2 a + 2\lambda b + c
\end{equation}

\begin{equation}
\left[ \begin{matrix}
2 & 1 & -2 & 1 \\
-3 & -2 & 3 & -1 \\
0 & 1 & 0 & 0 \\
1 & 0 & 0 & 0 
\end{matrix} \right]
\left[ \begin{matrix}
1 & 0 & 0 & 0 \\
-1 & 0 & 1 & 0 \\
0 & 1 & 0 & 0 \\
0 & -1 & 0 & 1 
\end{matrix} \right]
\left( \begin{matrix} A \\ B\\ C \\D\end{matrix}\right) = 
\left( \begin{matrix} a \\ b\\ c \\d\end{matrix}\right)
\end{equation}

\begin{equation}
\left[ \begin{matrix}
1 & -3 & 1 & 1 \\
-1 & 4 & -2 & -1 \\
-1 & 0 & 1 & 0 \\
1 & 0 & 0 & 0 
\end{matrix} \right]
\left( \begin{matrix} A \\ B\\ C \\D\end{matrix}\right) = 
\left( \begin{matrix} a \\ b\\ c \\d\end{matrix}\right)
\end{equation}

\begin{align}
a &= A-3B+C+D \nonumber \\
b &= 4B-A-2C-D \nonumber \\
c &= C-B \nonumber \\
d &= D
\end{align}

\begin{equation}
\left[ \begin{matrix}
1 & 0 & 0 & 0 \\
-1 & 0 & 1 & 0 \\
0 & 1 & 0 & 0 \\
0 & -1 & 0 & 1 
\end{matrix} \right]
\left( \begin{matrix} A \\ B\\ C \\D\end{matrix}\right) = \left[ \begin{matrix}
0 & 0 & 0 & 1 \\
0 & 0 & 1 & 0 \\
1 & 1 & 1 & 1 \\
3 & 2 & 1 & 0 
\end{matrix} \right]
\left( \begin{matrix} a \\ b\\ c \\d\end{matrix}\right)
\end{equation}